intermediate/Veritas.Intermediate.StoreSKC.fst
@@ -12,6 +12,10 @@ let store_contains_st_index (st:vstore) (s:slot_id{store_contains st s})
   : Lemma (s < Seq.length st.data)
   = ()
 
+let lemma_store_contains_empty (n:nat) (s:slot_id)
+  : Lemma (not (store_contains (empty_store n) s))
+  = ()
+
 let stored_key (st:vstore) (s:slot_id{store_contains st s}) : key
   = VStoreE?.k (Some?.v (get_slot st s))
 
@@ -26,11 +30,14 @@ let stored_value_matches_stored_key (st:vstore) (s:slot_id{store_contains st s})
 let add_method_of (st:vstore) (s:slot_id{store_contains st s}) : add_method
   = VStoreE?.am (Some?.v (get_slot st s))
 
+let has_key (k:key) (e:option vstore_entry) : bool
+  = match e with
+    | Some (VStoreE k' _ _) -> k = k'
+    | None -> false
+
 let lookup_key (st:vstore) (k:key) 
   : option vstore_entry
-  = let f ro = if None? ro then false
-               else let Some r = ro in r.k = k in
-    let s' = filter f st.data in
+  = let s' = filter (has_key k) st.data in
     if Seq.length s' = 0 then None
     else Seq.index s' 0 
 
@@ -40,47 +47,41 @@ let store_contains_key (st:vstore) (k:key) : bool
 let lemma_lookup_key_returns_k (st:vstore) (k:key) 
   : Lemma (requires (store_contains_key st k))
           (ensures (VStoreE?.k (Some?.v (lookup_key st k)) = k))
-  = let f ro = if None? ro then false
-               else let Some r = ro in r.k = k in
-    lemma_filter_correct1 f st.data 0
+  = lemma_filter_correct1 (has_key k) st.data 0
 
 let lemma_lookup_key_returns_None (st:vstore) (k:key)
   : Lemma (requires (lookup_key st k = None))
-          (ensures (let f ro = if None? ro then false
-                               else let Some r = ro in r.k = k in
-                    forall i. not (f (Seq.index st.data i))))
-  = let f ro = if None? ro then false
-               else let Some r = ro in r.k = k in
-    let s' = filter f st.data in
-    if Seq.length s' = 0 
-    then lemma_filter_all_not f st.data
-    else lemma_filter_correct1 f st.data 0
+          (ensures (forall i. not (has_key k (Seq.index st.data i))))
+  = if Seq.length (filter (has_key k) st.data) = 0 
+    then lemma_filter_all_not (has_key k) st.data
+    else lemma_filter_correct1 (has_key k) st.data 0
 
 let lemma_store_contains_key (st:vstore) (k:key)
   : Lemma (requires (exists s. stored_key st s = k))
           (ensures (store_contains_key st k))
-  = let f ro = if None? ro then false
-               else let Some r = ro in r.k = k in
-    lemma_filter_exists f st.data;
-    lemma_filter_correct1 f st.data 0
+  = lemma_filter_exists (has_key k) st.data;
+    lemma_filter_correct1 (has_key k) st.data 0
+
+let lemma_has_key (st:vstore) (s:slot_id) (k:key)
+  : Lemma (requires (has_key k (get_slot st s)))
+          (ensures (store_contains st s /\ stored_key st s = k))
+  = ()
 
 (* Opposite direction of previous lemma *)
 let lemma_store_contains_key_inv (st:vstore) (k:key)
   : Lemma (requires (store_contains_key st k))
           (ensures (exists s. stored_key st s = k))
-  = let f ro = if None? ro then false
-               else let Some r = ro in r.k = k in
-    let s' = filter f st.data in
+  = let s' = filter (has_key k) st.data in
     if Seq.length s' > 0 
     then 
-      let i = filter_index_map f st.data 0 in
-      assert (stored_key st i = k)
+      let i = filter_index_map (has_key k) st.data 0 in
+      lemma_has_key st i k
 
 let lemma_get_slot_lookup_key (st:vstore{st.is_map}) (s:slot_id) (k:key)
   : Lemma (requires (store_contains st s /\ stored_key st s = k))
           (ensures (get_slot st s = lookup_key st k))
-  = // relies on the fact that (filter f st.data) returns a unique elmt
-    admit()
+  = let s' = filter (has_key k) st.data in
+    lemma_filter_unique (has_key k) st.data s
 
 let stored_value_by_key (st:vstore) (k:key{store_contains_key st k})
   : value_type_of k
@@ -91,11 +92,11 @@ let add_method_of_by_key (st:vstore) (k:key{store_contains_key st k})
   : add_method
   = VStoreE?.am (Some?.v (lookup_key st k))
 
-(* Two cases where it's safe to add an entry (e) to the store (st) at s: 
-   * e.k is not in st
+(* Two cases where it's safe to add an entry (e) to the store (st) at slot s: 
+   * e.k is not in st and s is empty
    * e.k is already at s *)
 let compatible_entry (st:vstore) (s:st_index st) (e:vstore_entry) : Type
-  = not (store_contains_key st e.k) \/ 
+  = (not (store_contains st s) /\ not (store_contains_key st e.k)) \/ 
     (store_contains st s /\ stored_key st s = e.k) 
 
 let lemma_not_contains_key (st:vstore) (k:key) (s:slot_id{store_contains st s})
@@ -104,7 +105,7 @@ let lemma_not_contains_key (st:vstore) (k:key) (s:slot_id{store_contains st s})
   = ()
 
 let lemma_add_entry_case_1 (st:vstore) (s:st_index st) (e:vstore_entry)
-  : Lemma (requires (st.is_map /\ not (store_contains_key st e.k)))
+  : Lemma (requires (st.is_map /\ not (store_contains st s) /\ not (store_contains_key st e.k)))
           (ensures (is_map_f (Seq.upd st.data s (Some e))))
   = let l = Seq.upd st.data s (Some e) in
     let aux (i:seq_index l{Some? (Seq.index l i)})
@@ -140,22 +141,24 @@ let update_store
   = let Some (VStoreE k _ am) = get_slot st s in
     update_slot st s (VStoreE k v am) 
   
-let update_store_preserves_length 
-      (st:vstore) 
-      (s:slot_id{store_contains st s}) 
-      (v:value_type_of (stored_key st s)) 
+let update_store_preserves_length st s v 
   : Lemma (let st' = update_store st s v in
            Seq.length st.data = Seq.length st'.data)
   = ()
 
-let lemma_update_store_preserves_is_map (st:vstore) s v
+let lemma_update_store_preserves_is_map st s v
   : Lemma (let st' = update_store st s v in 
            st.is_map = st'.is_map)
   = ()
 
+let lemma_update_store_preserves_slots st s v
+  : Lemma (let st' = update_store st s v in
+           forall s. store_contains st s = store_contains st' s)
+  = ()
+
 let add_to_store 
       (st:vstore) 
-      (s:st_index st) 
+      (s:st_index st{not (store_contains st s)}) 
       (k:key) 
       (v:value_type_of k) 
       (am:add_method)
@@ -169,13 +172,13 @@ let add_to_store
     else VStore (Seq.upd st.data s (Some e)) false
 
 let lemma_add_to_store_is_map1 (st:vstore) s k v am
-  : Lemma (requires (not (store_contains_key st k)))
+  : Lemma (requires (not (store_contains st s) /\ not (store_contains_key st k)))
           (ensures (let st' = add_to_store st s k v am in 
                     st.is_map = st'.is_map))
   = ()
 
 let lemma_add_to_store_is_map2 (st:vstore) s k v am
-  : Lemma (requires (store_contains_key st k))
+  : Lemma (requires (not (store_contains st s) /\ store_contains_key st k))
           (ensures (let st' = add_to_store st s k v am in 
                     st'.is_map = false))
   = ()
@@ -215,7 +218,7 @@ let as_map (st:vstore{st.is_map}) : Spec.vstore =
   as_map_aux st.data
 
 let rec lemma_as_map_empty (n:nat) 
-  : Lemma (ensures (let st = VStore (Seq.create n None) true in
+  : Lemma (ensures (let st = empty_store n in
                      forall (k:key). as_map st k = None))
           (decreases n)
   = if n <> 0 
@@ -264,9 +267,7 @@ let lemma_as_map_slot_key_equiv (st:vstore{st.is_map}) (s:slot_id) (k:key)
 let rec lemma_as_map_aux_does_not_contain_key 
       (l:vstore_data) 
       (k:key) 
-  : Lemma (requires (let f ro = if None? ro then false
-                                else let Some r = ro in r.k = k in
-                     forall i. not (f (Seq.index l i)))) 
+  : Lemma (requires (forall i. not (has_key k (Seq.index l i)))) 
           (ensures (not (Spec.store_contains (as_map_aux l) k)))
           (decreases (Seq.length l))
   = let n = Seq.length l in
@@ -275,8 +276,9 @@ let rec lemma_as_map_aux_does_not_contain_key
       let l' = prefix l (n - 1) in
       lemma_as_map_aux_does_not_contain_key l' k
 
-let lemma_as_map_contains_key (st:vstore{st.is_map}) (k:key)
-  : Lemma (store_contains_key st k = Spec.store_contains (as_map st) k)
+let lemma_store_rel_contains_key (st:vstore) (st':Spec.vstore) (k:key)
+  : Lemma (requires (store_rel st st'))
+          (ensures (store_contains_key st k = Spec.store_contains st' k))
   = if store_contains_key st k
     then (
       lemma_store_contains_key_inv st k;
@@ -286,15 +288,13 @@ let lemma_as_map_contains_key (st:vstore{st.is_map}) (k:key)
         (fun s -> lemma_as_map_slot_key_equiv st s k)
     )
     else (
-      let f ro = if None? ro then false
-                 else let Some r = ro in r.k = k in
       lemma_lookup_key_returns_None st k;
       lemma_as_map_aux_does_not_contain_key st.data k
     )
 
-let lemma_as_map_stored_value (st:vstore{st.is_map}) (k:key)
-  : Lemma (requires (store_contains_key st k))
-          (ensures (stored_value_by_key st k = Spec.stored_value (as_map st) k))
+let lemma_store_rel_stored_value (st:vstore) (st':Spec.vstore) (k:key)
+  : Lemma (requires (store_rel st st' /\ store_contains_key st k))
+          (ensures (stored_value_by_key st k = Spec.stored_value st' k))
   = lemma_store_contains_key_inv st k;
     Classical.exists_elim 
       (stored_value_by_key st k = Spec.stored_value (as_map st) k) 
@@ -302,12 +302,85 @@ let lemma_as_map_stored_value (st:vstore{st.is_map}) (k:key)
       (fun s -> lemma_get_slot_lookup_key st s k; 
              lemma_as_map_slot_key_equiv st s k)
    
-let lemma_as_map_add_method_of (st:vstore{st.is_map}) (k:key)
-  : Lemma (requires (store_contains_key st k))
-          (ensures (add_method_of_by_key st k = Spec.add_method_of (as_map st) k))
+let lemma_store_rel_add_method_of (st:vstore) (st':Spec.vstore) (k:key)
+  : Lemma (requires (store_rel st st' /\ store_contains_key st k))
+          (ensures (add_method_of_by_key st k = Spec.add_method_of st' k))
   = lemma_store_contains_key_inv st k;
     Classical.exists_elim 
       (add_method_of_by_key st k = Spec.add_method_of (as_map st) k) 
       (Squash.get_proof (exists s. slot_key_equiv st s k)) 
       (fun s -> lemma_get_slot_lookup_key st s k; 
              lemma_as_map_slot_key_equiv st s k)
+
+let compatible_entry_prefix (st:vstore) (s:st_index st) (e:vstore_entry) (i:st_index st)
+  : Lemma (requires (compatible_entry st s e /\ s < i))
+          (ensures (compatible_entry (VStore (prefix st.data i) st.is_map) s e))
+          [SMTPat (compatible_entry (VStore (prefix st.data i) st.is_map) s e)]
+  = if not (store_contains st s)
+    then (
+      lemma_lookup_key_returns_None st e.k;
+      lemma_filter_all_not_inv (has_key e.k) (prefix st.data i)
+    )
+
+// TODO: sometimes this proof succeeds and sometimes Z3 times out
+let rec lemma_as_map_update (st:vstore{st.is_map}) (s:st_index st) (e:vstore_entry{compatible_entry st s e})
+  : Lemma (ensures (let m = as_map st in
+                    let m' = as_map (update_slot st s e) in
+                    m' e.k = Some (Spec.VStore e.v e.am) /\ (forall k. k <> e.k ==> m' k = m k))) 
+          (decreases (Seq.length st.data))
+  = let n = Seq.length st.data in
+    if n <> 0 
+    then
+      let stupd = update_slot st s e in
+      let l = prefix st.data (n - 1) in
+      let lupd = prefix stupd.data (n - 1) in
+      if s < n - 1
+      then ( 
+        let st' = VStore l true in
+        let stupd' = update_slot st' s e in      
+        lemma_as_map_update st' s e;
+        assert (Seq.equal stupd'.data lupd)
+      )
+      else ( // s = n - 1
+        assert (Seq.equal l lupd)
+      )
+
+let lemma_store_rel_update_store (st:vstore) (st':Spec.vstore) (s:slot_id) (k:key) (v:value_type_of k)
+  : Lemma (requires (store_rel st st' /\ slot_key_equiv st s k))
+          (ensures (store_rel (update_store st s v) (Spec.update_store st' k v)))
+  = let am = add_method_of st s in
+    lemma_as_map_update st s (VStoreE k v am)
+
+let lemma_store_rel_add_to_store (st:vstore) (st':Spec.vstore) (s:st_index st) (k:key) (v:value_type_of k) (am:add_method)
+  : Lemma (requires (store_rel st st' /\ not (store_contains st s) /\ not (Spec.store_contains st' k)))
+          (ensures (store_rel (add_to_store st s k v am) (Spec.add_to_store st' k v am)))
+  = lemma_as_map_update st s (VStoreE k v am)
+
+let rec lemma_as_map_evict (st:vstore{st.is_map}) (s:st_index st) (k:key)
+  : Lemma (requires (slot_key_equiv st s k))
+          (ensures (let m = as_map st in
+                    let m' = as_map (evict_from_store st s) in
+                    m' k = None /\ (forall k'. k' <> k ==> m' k' = m k'))) 
+          (decreases (Seq.length st.data))
+  = let n = Seq.length st.data in
+    if n <> 0 
+    then
+      let stupd = evict_from_store st s in
+      let l = prefix st.data (n - 1) in
+      let lupd = prefix stupd.data (n - 1) in
+      if s < n - 1
+      then ( 
+        let st' = VStore l true in
+        let stupd' = evict_from_store st' s in      
+        lemma_as_map_evict st' s k;
+        assert (Seq.equal stupd'.data lupd)
+      )
+      else (  // s = n - 1
+        assert (Seq.equal lupd l);
+        lemma_as_map_aux_does_not_contain_key l k
+      )
+
+let lemma_store_rel_evict_from_store (st:vstore) (st':Spec.vstore) (s:st_index st) (k:key)
+  : Lemma (requires (store_rel st st' /\ slot_key_equiv st s k))
+          (ensures (store_rel (evict_from_store st s) (Spec.evict_from_store st' k)))
+  = lemma_as_map_evict st s k
