intermediate/Veritas.Intermediate.StoreSKC.fsti
@@ -5,6 +5,7 @@ open Veritas.Record
 open Veritas.SeqAux
 
 module Spec = Veritas.Verifier
+module FE = FStar.FunctionalExtensionality
 
 let slot_id = nat
 let add_method = Veritas.Verifier.add_method
@@ -31,6 +32,8 @@ let elim_is_map_f (s:vstore_data)
 type vstore = 
   | VStore: data:vstore_data -> is_map:bool{is_map ==> is_map_f data} -> vstore
 
+let empty_store (n:nat) :vstore = VStore (Seq.create n None) true
+
 let st_index (st:vstore) = seq_index st.data
 
 val store_contains (st:vstore) (s:slot_id) : bool
@@ -38,6 +41,10 @@ val store_contains (st:vstore) (s:slot_id) : bool
 val store_contains_st_index (st:vstore) (s:slot_id{store_contains st s})
   : Lemma (s < Seq.length st.data)
           [SMTPat (store_contains st s)] 
+
+val lemma_store_contains_empty (n:nat) (s:slot_id)
+  : Lemma (not (store_contains (empty_store n) s))
+          [SMTPat (store_contains (empty_store n) s)]
 
 val stored_key (st:vstore) (s:slot_id{store_contains st s}) : key
 
@@ -83,9 +90,17 @@ val lemma_update_store_preserves_is_map
            st.is_map = st'.is_map)
           [SMTPat (update_store st s v)]
 
+val lemma_update_store_preserves_slots
+      (st:vstore) 
+      (s:slot_id{store_contains st s}) 
+      (v:value_type_of (stored_key st s))
+  : Lemma (let st' = update_store st s v in
+           forall s. store_contains st s = store_contains st' s)
+          [SMTPat (update_store st s v)]
+
 val add_to_store 
       (st:vstore) 
-      (s:st_index st) 
+      (s:st_index st{not (store_contains st s)})
       (k:key) 
       (v:value_type_of k) 
       (am:add_method)
@@ -100,7 +115,7 @@ val lemma_add_to_store_is_map1
       (k:key) 
       (v:value_type_of k) 
       (am:add_method)
-  : Lemma (requires (not (store_contains_key st k)))
+  : Lemma (requires (not (store_contains st s) /\ not (store_contains_key st k)))
           (ensures (let st' = add_to_store st s k v am in 
                     st.is_map = st'.is_map))
           [SMTPat (add_to_store st s k v am)]
@@ -111,7 +126,7 @@ val lemma_add_to_store_is_map2
       (k:key) 
       (v:value_type_of k) 
       (am:add_method)
-  : Lemma (requires (store_contains_key st k))
+  : Lemma (requires (not (store_contains st s) /\ store_contains_key st k))
           (ensures (let st' = add_to_store st s k v am in 
                     st'.is_map = false))
           [SMTPat (add_to_store st s k v am)]
@@ -142,13 +157,8 @@ val lemma_slot_key_equiv_update_store
 (* convert a slot-indexed store to a key-indexed store *)
 val as_map (st:vstore{st.is_map}) : Spec.vstore
 
-let lemma_is_map_empty (n:nat) 
-  : Lemma (is_map_f (Seq.create n (None #vstore_entry)))
-          [SMTPat (Seq.create n (None #vstore_entry))]
-  = ()
-
 val lemma_as_map_empty (n:nat) 
-  : Lemma (ensures (let st = VStore (Seq.create n None) true in
+  : Lemma (ensures (let st = empty_store n in
                      forall (k:key). as_map st k = None))
           (decreases n)
 
@@ -159,16 +169,36 @@ val lemma_as_map_slot_key_equiv (st:vstore{st.is_map}) (s:slot_id) (k:key)
                     add_method_of st s = Spec.add_method_of (as_map st) k))
           [SMTPat (slot_key_equiv st s k)]
 
-val lemma_as_map_contains_key (st:vstore{st.is_map}) (k:key)
-  : Lemma (store_contains_key st k = Spec.store_contains (as_map st) k)
-          [SMTPat (store_contains_key st k)]
+(* Relation between stores *)
+let store_rel (st:vstore) (st':Spec.vstore) : Type = 
+  st.is_map /\ FE.feq st' (as_map st)
 
-val lemma_as_map_stored_value (st:vstore{st.is_map}) (k:key)
-  : Lemma (requires (store_contains_key st k))
-          (ensures (stored_value_by_key st k = Spec.stored_value (as_map st) k))
-          [SMTPat (stored_value_by_key st k)]
+val lemma_store_rel_contains_key (st:vstore) (st':Spec.vstore) (k:key)
+  : Lemma (requires (store_rel st st'))
+          (ensures (store_contains_key st k = Spec.store_contains st' k))
+          [SMTPat (store_contains_key st k); SMTPat (Spec.store_contains st' k)]
 
-val lemma_as_map_add_method_of (st:vstore{st.is_map}) (k:key)
-  : Lemma (requires (store_contains_key st k))
-          (ensures (add_method_of_by_key st k = Spec.add_method_of (as_map st) k))
-          [SMTPat (add_method_of_by_key st k)]
+val lemma_store_rel_stored_value (st:vstore) (st':Spec.vstore) (k:key)
+  : Lemma (requires (store_rel st st' /\ store_contains_key st k))
+          (ensures (stored_value_by_key st k = Spec.stored_value st' k))
+          [SMTPat (stored_value_by_key st k); SMTPat (Spec.stored_value st' k)]
+
+val lemma_store_rel_add_method_of (st:vstore) (st':Spec.vstore) (k:key)
+  : Lemma (requires (store_rel st st' /\ store_contains_key st k))
+          (ensures (add_method_of_by_key st k = Spec.add_method_of st' k))
+          [SMTPat (add_method_of_by_key st k); SMTPat (Spec.add_method_of st' k)]
+
+val lemma_store_rel_update_store (st:vstore) (st':Spec.vstore) (s:slot_id) (k:key) (v:value_type_of k)
+  : Lemma (requires (store_rel st st' /\ slot_key_equiv st s k))
+          (ensures (store_rel (update_store st s v) (Spec.update_store st' k v)))
+          [SMTPat (update_store st s v); SMTPat (Spec.update_store st' k v)]
+
+val lemma_store_rel_add_to_store (st:vstore) (st':Spec.vstore) (s:st_index st) (k:key) (v:value_type_of k) (am:add_method)
+  : Lemma (requires (store_rel st st' /\ not (store_contains st s) /\ not (Spec.store_contains st' k)))
+          (ensures (store_rel (add_to_store st s k v am) (Spec.add_to_store st' k v am)))
+          [SMTPat (add_to_store st s k v am); SMTPat (Spec.add_to_store st' k v am)]
+
+val lemma_store_rel_evict_from_store (st:vstore) (st':Spec.vstore) (s:st_index st) (k:key)
+  : Lemma (requires (store_rel st st' /\ slot_key_equiv st s k))
+          (ensures (store_rel (evict_from_store st s) (Spec.evict_from_store st' k)))
+          [SMTPat (evict_from_store st s); SMTPat (Spec.evict_from_store st' k)]
