Veritas.SeqAux.fsti
@@ -111,12 +111,20 @@ val lemma_filter_correct_all (#a:eqtype) (f:a -> bool) (s:seq a):
         (ensures (forall (i:(seq_index (filter f s))). f (index (filter f s) i) = true))
 
 val lemma_filter_all_not (#a:eqtype) (f:a -> bool) (s:seq a):
-  Lemma (requires filter f s `Seq.equal` empty)
-        (ensures forall (i:seq_index s). not (f (Seq.index s i)))
+  Lemma (requires filter f s `equal` empty)
+        (ensures forall (i:seq_index s). not (f (index s i)))
+
+val lemma_filter_all_not_inv (#a:eqtype) (f:a->bool) (s:seq a)
+  : Lemma (requires (forall (i:seq_index s). not (f (index s i))))
+          (ensures (equal (filter f s) empty))
 
 val lemma_filter_exists (#a:eqtype) (f:a -> bool) (s:seq a):
   Lemma (requires (exists (i:seq_index s). f (index s i)))
         (ensures (length (filter f s) > 0))
+
+val lemma_filter_unique (#a:eqtype) (f:a->bool) (s: seq a) (i:seq_index s)
+  : Lemma (requires (f (index s i) /\ (forall j. j <> i ==> not (f (index s j)))))
+          (ensures (filter f s = create 1 (index s i)))
 
 (* mapping from filtered subseq to satisfying indexes *)
 val filter_index_map (#a:eqtype) (f:a -> bool) (s:seq a) (i:seq_index (filter f s)):
